concurrency/sc_drf/Coarse2Fine_safety.v
@@ -35,6 +35,7 @@ Require Import VST.concurrency.sc_drf.x86_erasure.
 Require Import VST.concurrency.sc_drf.x86_inj.
 Require Import VST.concurrency.sc_drf.fineConc_safe.
 Require Import VST.concurrency.sc_drf.SC_erasure.
+Require Import VST.concurrency.sc_drf.SC_spinlock_safe.
 
 Require Import Coqlib.
 Require Import VST.msl.Coqlib2.
